src/crypto/aes/aes-x64/gcm_helpers.i.dfy
@@ -28,4 +28,83 @@ lemma lemma_BitwiseAdd32()
     reveal_BitwiseAdd32();
 }
 
+// It's not clear to me what is the best way to allow proof.
+// 0b00010000 
+function uint8Tobv8(b : uint8) : bv8 { b as bv8 }
+
+/* Whoa, where are bit vectors specified?
+predicate isbv8eq0(b : bv8) {
+  b[0] == 0
+}
+
+method CL_MUL_SHIFT(a : bv64, b : bv64) returns (r : bv128)
+{
+   var a' := a;
+   var b' := b;
+   r := 0;
+    while b' != 0
+  {
+     if ((a' & 1) != 0) {
+          r := r ^ b';
+     }
+    a' := a' >> 1;
+    b' := b' << 1;
+ }
+}
+
+method CL_MUL(src1 : bv128, src2 : bv128, imm8 : bv8) returns (dest : bv128) 
+{
+  var temp1 : bv64;
+  var temp2 : bv128;
+
+  if (imm8[0] == 0) {
+    temp1 := src1[63:0];
+  } else {
+    temp1 := src1[127:64];
+  }
+
+  if (imm8[4] == 0) {
+    temp2 := src2[63:0];
+  } else {
+    temp2 := src2[127:64];
+  }
+
+  var dest : bv128;
+  var i := 0;
+  var tempb : bv128;
+  while (i <= 63) {
+   tempb[i] := (temp1[0] & temp2[i]);
+   var j := 1; 
+   while (j <= i) {
+    tempb[i] := tempb [i] ^ (temp1[j] & temp2[i - j]);
+    j := j + 1;
+   }    
+   dest[i] := tempb[i];
+   i := i + 1;
+  }      
+
+  i := 64; 
+  while (i <= 126) {
+     tempb[i] := 0;
+     j := i - 63; 
+     while (j >= 63) {
+       tempb[i] := tempb[i] ^ (temp1[j] & temp2[i - j]);
+       j := j + 1;
+     }
+     dest[i] := tempb[i];
+     i := i + 1;
+  } 
+  dest[127] := 0;
+}
+*/
+
+
+// Find a new index that is open, 32 bit. 
+// Assume the rest after that is clear, which may cause proof issues.
+function FrameMax(f : Frame, upto : int) : int 
+  decreases |f|;
+{
+  if !(upto in f) then upto else FrameMax(map i | i in f && i != upto :: f[i], upto + 1)
+}
+
 }
