src/arch/x64/printMasm.s.dfy
@@ -247,7 +247,7 @@ method printIns(ins:ins)
         case VPSLLDQ(dst, src, count) => print ("  vpslldq "); printOprnd(dst); print(", "); printOprnd(src); print(", "); printOprnd(count); print("\n");
 
         case MOVDQU(dst, src) => print ("  movdqu "); printXmmOprnd(dst); print(", "); printXmmOprnd(src); print("\n");
-        case MOVDxmmr32(dst, src) => print ("  movd "); printXmmOprnd(dst); print(", "); printOprnd(src); print("\n");
+        case MOVD_xmm_rmm32(dst, src) => print ("  movd "); printXmmOprnd(dst); print(", "); printOprnd(src); print("\n");
         case PCLMULQDQ(dst, src, imm8) => print ("  pclmulqdq "); print(", "); printOprnd(dst); print(", "); printOprnd(src); print(","); printOprnd(imm8); print("\n");
         case VPCLMULQDQ(dst, src1, src2, imm8)  => print ("  vpclmulqdq "); printOprnd(dst); print(", "); printOprnd(src1); print(", "); printOprnd(src2); print(", "); printOprnd(imm8); print("\n");
         case VMOVDAQ(dst, src)        => print ("  vmovdqa "); printXmmOprnd(dst); print(", "); printOprnd(src); print("\n");          
@@ -259,6 +259,8 @@ method printIns(ins:ins)
         case PSLLD (dst, imm8)        => print ("  pslld ");  printOprnd(dst); print(", "); printOprnd(imm8); print("\n");
         case PSRLDQ(dst, imm8)        => print ("  psrldq "); printOprnd(dst); print(", "); printOprnd(imm8); print("\n");
         case PSRLD (dst, imm8)        => print ("  psrld ");  printOprnd(dst); print(", "); printOprnd(imm8); print("\n");
+        case PUSH (src)               => print ("  push  ");  printOprnd(src); print("\n");
+        case POP (dst)                => print ("  pop  ");   printOprnd(dst); print("\n");
 }
 
 method printBlock(b:codes, n:int) returns(n':int)
